theories/TRAKHTENBROT/fo_terms.v
@@ -12,14 +12,11 @@ Require Import List Arith Lia.
 From Undecidability.Shared.Libs.DLW.Utils
   Require Import utils_tac utils_list utils_nat finite.
 
-From Undecidability.Shared.Libs.DLW.Wf
-  Require Import acc_irr.
-
 From Undecidability.Shared.Libs.DLW.Vec 
   Require Import pos vec.
 
 From Undecidability.TRAKHTENBROT
-  Require Import notations fol_ops utils.
+  Require Import notations utils fol_ops fo_sig.
 
 Set Implicit Arguments.
 
@@ -29,173 +26,34 @@ Local Hint Resolve in_vec_list in_vec_pos.
 
 Section first_order_terms.
 
-  Variable (var sym : Type)        (* a type of variables and symbols *)
-           (sym_ar : sym -> nat).  (* arities for symbols *)
+  Variable (syms : Type) (ar_syms : syms -> nat).
 
   Unset Elimination Schemes.       (* we do not want the autogen recursors *)
 
   (** The Type of first order terms over signature s *)
 
   Inductive fo_term : Type :=
-    | in_var : var -> fo_term
-    | in_fot : forall s, vec fo_term (sym_ar s) -> fo_term.
+    | in_var : nat -> fo_term
+    | in_fot : forall s, vec fo_term (ar_syms s) -> fo_term.
 
   Set Elimination Schemes.
 
   Section fo_term_rect.
-
-    (** We build a Type level dependent recursor together with
-        a fixpoint equation *)
-
-    Let sub_fo_term x t := 
-      match t with 
-        | in_var _    => False 
-        | @in_fot s v => in_vec x v 
-      end.  
-
-    (** This proof has to be carefully crafted for guardness *)
- 
-    Let Fixpoint Acc_sub_fo_term t : Acc sub_fo_term t.
-    Proof.
-      destruct t as [ x | s v ]; constructor 1; simpl.
-      + intros _ [].
-      + intros x.
-        revert v; generalize (sym_ar s).
-        induction v as [ | n y w IHw ].
-        * destruct 1.
-        * intros [ H | H ].
-          - rewrite <- H; apply Acc_sub_fo_term.
-          - apply IHw, H.
-    Qed.
-
-    (** This is a Type level (_rect) dependent recursor with induction
-        hypothesis using Prop level in_vec *) 
-
-    Variable (P   : fo_term -> Type)
-             (HP0 : forall x, P (in_var x))
-             (IHP : forall s v, (forall t, in_vec t v -> P t) -> P (@in_fot s v)).
-
-    Let Fixpoint Fix_IHP t (Ht : Acc sub_fo_term t) { struct Ht } : P t :=
-      match t as t' return Acc sub_fo_term t'-> P t' with
-        | in_var x    => fun _  => HP0 x
-        | @in_fot s v => fun Ht => @IHP s v (fun x Hx => @Fix_IHP x (Acc_inv Ht _ Hx))
-      end Ht.
-
-    Let Fix_IHP_fix t Ht :
-        @Fix_IHP t Ht 
-      = match t as t' return Acc sub_fo_term t' -> _ with 
-          | in_var x    => fun _   => HP0 x
-          | @in_fot s v => fun Ht' => @IHP s v (fun y H => Fix_IHP (Acc_inv Ht' H)) 
-        end Ht.
-    Proof. destruct Ht; reflexivity. Qed.
-
-    Definition fo_term_rect' t : P t.
-    Proof. apply Fix_IHP with (1 := Acc_sub_fo_term t). Defined.
-
-    Hypothesis IHP_ext : forall s v f g, (forall y H, f y H = g y H) -> @IHP s v f = IHP v g.
-
-    Let Fix_IHP_Acc_irr : forall t f g, @Fix_IHP t f = Fix_IHP g.
-    Proof.
-      apply Acc_irrelevance.
-      intros [] f g H; auto; apply IHP_ext; auto.
-    Qed.
-
-    Theorem fo_term_rect_fix' s v : 
-            fo_term_rect' (@in_fot s v) = @IHP s v (fun t _ => fo_term_rect' t).
-    Proof.
-      unfold fo_term_rect' at 1.
-      rewrite Fix_IHP_fix.
-      apply IHP_ext.
-      intros; apply Fix_IHP_Acc_irr.
-    Qed.
-
-  End fo_term_rect.
-
-  Definition fo_term_rec' (P : _ -> Set) := @fo_term_rect' P.
-  Definition fo_term_ind' (P : _ -> Prop) := @fo_term_rect' P.
-
-  Section fo_term_pos_rect.
-
-    (** This one is nicer to compute *)
    
     Variable (P   : fo_term -> Type)
              (HP0 : forall x, P (in_var x))
              (IHP : forall s v, (forall p, P (vec_pos v p)) -> P (@in_fot s v)).
 
-    Fixpoint fo_term_pos_rect t : P t :=
+    Fixpoint fo_term_rect t : P t :=
       match t with
         | in_var x => HP0 x 
-        | in_fot v => IHP v (fun p => fo_term_pos_rect (vec_pos v p))
+        | in_fot v => IHP v (fun p => fo_term_rect (vec_pos v p))
       end.
 
-  End fo_term_pos_rect.
+  End fo_term_rect.
 
-  Definition fo_term_rect (P : _ -> Type) := @fo_term_pos_rect P.
   Definition fo_term_rec (P : _ -> Set) := @fo_term_rect P.
   Definition fo_term_ind (P : _ -> Prop) := @fo_term_rect P.
- 
-  Section fo_term_recursion.
-
-    (** We specialize the nice recursor to fixed output type.
-        The fixpoint equation are better behaved *)
-
-    Variable (X : Type)
-             (F0 : var -> X)
-             (F  : forall s, vec fo_term (sym_ar s) -> vec X (sym_ar s) -> X).
-
-    Definition fo_term_recursion : fo_term -> X.
-    Proof.
-      induction 1 as [ x | s v IHv ].
-      + exact (F0 x).
-      + apply (@F s v), vec_set_pos, IHv.
-    Defined.
-
-    Theorem fo_term_recursion_fix_0 x :
-      fo_term_recursion (in_var x) = F0 x.
-    Proof. reflexivity. Qed.
-
-    Theorem fo_term_recursion_fix_1 s v :
-      fo_term_recursion (@in_fot s v) = F v (vec_map fo_term_recursion v).
-    Proof.
-      unfold fo_term_recursion at 1.
-      simpl; f_equal; apply vec_pos_ext; intro; rew vec.
-    Qed.
-
-  End fo_term_recursion.
-
-  (** We can now define eg the size of terms easily with the
-      corresponding fixpoint equation *)
-
-  Fixpoint fo_term_size c t :=
-    match t with
-      | in_var _    => 1
-      | @in_fot s v => c s + vec_sum (vec_map (fo_term_size c) v)
-    end.
-
-  Fact fo_term_size_fix_0 c x : fo_term_size c (in_var x) = 1.
-  Proof. trivial. Qed.
-  
-  Fact fo_term_size_fix_1 c s v :
-         fo_term_size c (@in_fot s v) = c s + vec_sum (vec_map (fo_term_size c) v).
-  Proof. trivial. Qed.
-
-  (*
-
-  Definition fo_term_size' (c : sym -> nat) : fo_term -> nat.
-  Proof.
-    induction 1 as [ _ | s _ w ] using fo_term_recursion.
-    + exact 1.
-    + exact (c s+vec_sum w).
-  Defined.
-
-  Fact fo_term_size_fix_0' c x : fo_term_size' c (in_var x) = 1.
-  Proof. apply fo_term_recursion_fix_0. Qed.
-  
-  Fact fo_term_size_fix_1' c s v :
-         fo_term_size' c (@in_fot s v) = c s + vec_sum (vec_map (fo_term_size' c) v).
-  Proof. apply fo_term_recursion_fix_1. Qed.
-
-  *)
 
   Fixpoint fo_term_vars t :=
     match t with 
@@ -209,26 +67,6 @@ Section first_order_terms.
   Fact fo_term_vars_fix_1 s v : fo_term_vars (@in_fot s v) = flat_map fo_term_vars (vec_list v).
   Proof. simpl; rewrite vec_list_vec_map, <- flat_map_concat_map; auto. Qed.
 
-  (*
-
-  Definition fo_term_vars : fo_term -> list var.
-  Proof.
-    induction 1 as [ x | s _ w ] using fo_term_recursion.
-    + exact (x::nil).
-    + exact (concat (vec_list w)).
-  Defined.
-
-  Fact fo_term_vars_fix_0 x : fo_term_vars (in_var x) = x :: nil.
-  Proof. apply fo_term_recursion_fix_0. Qed.
-
-  Fact fo_term_vars_fix_2 s v : fo_term_vars (@in_fot s v) = concat (vec_list (vec_map fo_term_vars v)).
-  Proof. apply fo_term_recursion_fix_1. Qed.
-
-  Fact fo_term_vars_fix_1 s v : fo_term_vars (@in_fot s v) = flat_map fo_term_vars (vec_list v).
-  Proof. rewrite fo_term_vars_fix_2, vec_list_vec_map, <- flat_map_concat_map; auto. Qed.
-
-  *)
-
   Fixpoint fo_term_syms t :=
     match t with 
       | in_var x    => nil
@@ -241,47 +79,10 @@ Section first_order_terms.
   Fact fo_term_syms_fix_1 s v : fo_term_syms (@in_fot s v) = s::flat_map fo_term_syms (vec_list v).
   Proof. simpl; rewrite vec_list_vec_map, <- flat_map_concat_map; auto. Qed.
 
-   (*
-
-  Definition fo_term_syms : fo_term -> list sym.
-  Proof.
-    induction 1 as [ x | s _ w ] using fo_term_recursion.
-    + exact nil.
-    + exact (s::concat (vec_list w)).
-  Defined.
-
-  Fact fo_term_syms_fix_0 x : fo_term_syms (in_var x) = nil.
-  Proof. apply fo_term_recursion_fix_0. Qed.
-
-  Fact fo_term_syms_fix_2 s v : fo_term_syms (@in_fot s v) = s::concat (vec_list (vec_map fo_term_syms v)).
-  Proof. apply fo_term_recursion_fix_1. Qed.
-
-  Fact fo_term_syms_fix_1 s v : fo_term_syms (@in_fot s v) = s::flat_map fo_term_syms (vec_list v).
-  Proof. rewrite fo_term_syms_fix_2, vec_list_vec_map, <- flat_map_concat_map; auto. Qed.
-
-  *)
-
-End first_order_terms.
-
-Arguments in_var { var sym sym_ar }.
-
-Create HintDb fo_term_db.
-Tactic Notation "rew" "fot" := autorewrite with fo_term_db.
-
-Hint Rewrite fo_term_vars_fix_0 fo_term_vars_fix_1 
-             fo_term_syms_fix_0 fo_term_syms_fix_1 : fo_term_db.
-
-Section fo_term_subst.
-
-  Variable (sym : Type) (sym_ar : sym -> nat)
-           (X Y : Type).
-
-  Implicit Type (σ : X -> fo_term Y sym_ar).
-
-  Fixpoint fo_term_subst σ (t : fo_term X sym_ar) :=
+  Fixpoint fo_term_subst σ t :=
     match t with 
-      | in_var x   => σ x
-      | in_fot s v => in_fot s (vec_map (fo_term_subst σ) v)
+      | in_var x => σ x
+      | in_fot v => in_fot (vec_map (fo_term_subst σ) v)
     end.
 
   Notation "t ⟬ σ ⟭" := (fo_term_subst σ t).
@@ -289,54 +90,70 @@ Section fo_term_subst.
   Fact fo_term_subst_fix_0 σ x : (in_var x)⟬σ⟭  = σ x.
   Proof. trivial. Qed.
 
-  Fact fo_term_subst_fix_1 σ s v : (in_fot s v)⟬σ⟭ 
-                                  = in_fot s (vec_map (fo_term_subst σ) v).
+  Fact fo_term_subst_fix_1 σ s v : 
+          (@in_fot s v)⟬σ⟭  = in_fot (vec_map (fo_term_subst σ) v).
   Proof. trivial. Qed.
-
-  (*
-
-  Definition fo_term_subst σ : fo_term X sym_ar -> fo_term Y sym_ar.
-  Proof.
-    induction 1 as [ x | s _ w ] using fo_term_recursion.
-    + apply σ, x.
-    + exact (in_fot s w).
-  Defined.
-
-  Notation "t ⟬ σ ⟭" := (fo_term_subst σ t).
-
-  Fact fo_term_subst_fix_0 σ x : (in_var x)⟬σ⟭  = σ x.
-  Proof. apply fo_term_recursion_fix_0. Qed.
-
-  Fact fo_term_subst_fix_1 σ s v : (in_fot s v)⟬σ⟭ 
-                                  = in_fot s (vec_map (fo_term_subst σ) v).
-  Proof. apply fo_term_recursion_fix_1. Qed.
-
-  *)
-
-  Opaque fo_term_subst.
-
-  Hint Rewrite fo_term_subst_fix_0 fo_term_subst_fix_1 : fo_term_db.
 
   Fact fo_term_subst_ext f g t : 
      (forall x, In x (fo_term_vars t) -> f x = g x) -> t⟬f⟭ = t⟬g⟭.
   Proof.
-    induction t as [ | s v IHv ]; intros Hfg; rew fot.
-    + apply Hfg; rew fot; simpl; auto.
-    + simpl; f_equal; apply vec_map_ext.
+    induction t as [ | s v IHv ]; intros Hfg; simpl.
+    + apply Hfg; simpl; auto.
+    + f_equal; apply vec_map_ext.
       intros x Hx. 
       apply in_vec_list, vec_list_inv in Hx.
       destruct Hx as (p & ->).
       apply IHv.
-      intros y Hy; apply Hfg; rew fot. 
-      apply in_flat_map; exists (vec_pos v p).
+      intros y Hy; apply Hfg.
+      rewrite fo_term_vars_fix_1, in_flat_map.
+      exists (vec_pos v p).
       split; auto; apply in_vec_list; auto.
   Qed.
 
+  Section fo_term_subst_comp.
+
+    Variables (f g : nat -> fo_term).
+
+    Fact fo_term_subst_comp t : t⟬f⟭ ⟬g⟭ = t⟬fun x => (f x)⟬g⟭ ⟭ . 
+    Proof.
+      induction t; simpl; auto.
+      rewrite vec_map_map; f_equal.
+      apply vec_pos_ext; intros p; rew vec.
+    Qed.
+
+  End fo_term_subst_comp.
+
+End first_order_terms.
+
+Notation fol_term := (fun Σ => fo_term (ar_syms Σ)).
+
+Arguments in_var { _ _ }.
+Arguments in_fot { _ _ }.
+
+Create HintDb fo_term_db.
+Tactic Notation "rew" "fot" := autorewrite with fo_term_db.
+
+Hint Rewrite fo_term_vars_fix_0   fo_term_vars_fix_1 
+             fo_term_syms_fix_0   fo_term_syms_fix_1 
+             fo_term_subst_fix_0  fo_term_subst_fix_1 
+             fo_term_subst_comp 
+           : fo_term_db.
+
+Notation "t ⟬ σ ⟭" := (fo_term_subst σ t).
+
+Section fo_term_extra.
+
+  Variable (Σ : fo_signature).
+
+  Notation 𝕋 := (fol_term Σ).
+
+  Implicit Type t : 𝕋.
+
   Section map.
 
-    Variable (f : X -> Y).
+    Variable (f : nat -> nat).
 
-    Fixpoint fo_term_map (t : fo_term X sym_ar) := 
+    Fixpoint fo_term_map t := 
       match t with
         | in_var x   => in_var (f x)
         | in_fot s v => in_fot s (vec_map fo_term_map v)
@@ -348,24 +165,6 @@ Section fo_term_subst.
     Fact fo_term_map_fix_1 s v : 
          fo_term_map (in_fot s v) = in_fot s (vec_map fo_term_map v).
     Proof. trivial. Qed.
-
-    (*
-
-    Definition fo_term_map : fo_term X sym_ar -> fo_term Y sym_ar.
-    Proof.
-      induction 1 as [ x | s _ w ] using fo_term_recursion.
-      + exact (in_var (f x)).
-      + exact (in_fot s w).
-    Defined.
-
-    Fact fo_term_map_fix_0 x : fo_term_map (in_var x) = in_var (f x).
-    Proof. apply fo_term_recursion_fix_0. Qed.
-
-    Fact fo_term_map_fix_1 s v : 
-         fo_term_map (in_fot s v) = in_fot s (vec_map fo_term_map v).
-    Proof. apply fo_term_recursion_fix_1. Qed.
-
-    *)
 
   End map.
 
@@ -379,8 +178,9 @@ Section fo_term_subst.
     apply vec_pos_ext; intro; rew vec. 
   Qed.
 
-  Fact fo_term_map_ext f g t : (forall x, In x (fo_term_vars t) -> f x = g x)
-                             -> fo_term_map f t = fo_term_map g t.
+  Fact fo_term_map_ext f g t : 
+           (forall x, In x (fo_term_vars t) -> f x = g x)
+        -> fo_term_map f t = fo_term_map g t.
   Proof.
     intros Hfg. 
     do 2 rewrite <- fo_term_subst_map.
@@ -451,55 +251,39 @@ Section fo_term_subst.
           apply in_vec_list, in_vec_pos.
   Qed.
 
-End fo_term_subst.
+End fo_term_extra.
 
-Opaque fo_term_map fo_term_subst.
+Arguments fo_term_vars {_ _}.
+Arguments fo_term_syms {_ _}.
 
-Hint Rewrite fo_term_subst_fix_0 fo_term_subst_fix_1
-             fo_term_map_fix_0 fo_term_map_fix_1 : fo_term_db.
+Opaque fo_term_map.
 
-Notation "t ⟬ σ ⟭" := (fo_term_subst σ t).
+Hint Rewrite fo_term_map_fix_0 fo_term_map_fix_1 
+           : fo_term_db.
 
-Section fo_term_subst_comp.
-
-  Variables (sym : Type) (sym_ar : sym -> nat) (X Y Z : Type) 
-            (f : X -> fo_term Y sym_ar) 
-            (g : Y -> fo_term Z sym_ar).
-
-  Fact fo_term_subst_comp t : t⟬f⟭ ⟬g⟭ = t⟬fun x => (f x)⟬g⟭ ⟭ . 
-  Proof.
-    induction t; rew fot; auto; rew fot.
-    rewrite vec_map_map; f_equal.
-    apply vec_pos_ext; intros p; rew vec.
-  Qed.
-
-End fo_term_subst_comp.
-
-Hint Rewrite fo_term_subst_comp : fo_term_db.
-
-Definition fo_term_subst_lift s ar (σ : nat -> @fo_term nat s ar) n :=
+Definition fo_term_subst_lift Σ (σ : nat -> fol_term Σ) n :=
   match n with 
     | 0   => in_var 0
     | S n => fo_term_map S (fo_term_subst σ (in_var n))
   end.
 
-Arguments fo_term_subst_lift {s ar } σ n /.
+Arguments fo_term_subst_lift {Σ} σ n /.
 
 Notation "⇡ σ" := (fo_term_subst_lift σ).
 
 Section semantics.
 
-  Variable (sym : Type) (sym_ar : sym -> nat) (X : Type)
-           (M : Type) (sem_sym : forall s, vec M (sym_ar s) -> M).
+  Variable (Σ : fo_signature) 
+           (X : Type) (M : fo_model Σ X).
 
-  Notation 𝕋 := (fo_term X sym_ar).
+  Notation 𝕋 := (fol_term Σ).
 
-  Implicit Type φ : X -> M.
+  Implicit Type φ : nat -> X.
 
   Fixpoint fo_term_sem φ (t : 𝕋) :=
     match t with
       | in_var x   => φ x
-      | in_fot s v => sem_sym (vec_map (fo_term_sem φ) v)
+      | in_fot s v => fom_syms M s (vec_map (fo_term_sem φ) v)
     end.
 
   Notation "⟦ t ⟧" := (fun φ => @fo_term_sem φ t).
@@ -507,27 +291,8 @@ Section semantics.
   Fact fo_term_sem_fix_0 φ n : ⟦in_var n⟧ φ = φ n.
   Proof. trivial. Qed.
 
-  Fact fo_term_sem_fix_1 φ s v : ⟦in_fot s v⟧ φ = sem_sym (vec_map (fun t => ⟦t⟧ φ) v).
+  Fact fo_term_sem_fix_1 φ s v : ⟦in_fot s v⟧ φ = fom_syms M s (vec_map (fun t => ⟦t⟧ φ) v).
   Proof. trivial. Qed.
-
-  (*
-
-  Definition fo_term_sem φ : 𝕋 -> M.
-  Proof.
-    induction 1 as [ x | s _ w ] using fo_term_recursion.
-    + exact (φ x).
-    + exact (sem_sym w).
-  Defined.
-
-  Notation "⟦ t ⟧" := (fun φ => @fo_term_sem φ t).
-
-  Fact fo_term_sem_fix_0 φ n : ⟦in_var n⟧ φ = φ n.
-  Proof. apply fo_term_recursion_fix_0. Qed.
-
-  Fact fo_term_sem_fix_1 φ s v : ⟦in_fot s v⟧ φ = sem_sym (vec_map (fun t => ⟦t⟧ φ) v).
-  Proof. apply fo_term_recursion_fix_1. Qed.
-
-  *)
 
   Opaque fo_term_sem.
 
@@ -562,14 +327,14 @@ Hint Rewrite fo_term_sem_fix_0 fo_term_sem_fix_1 fo_term_sem_subst : fo_term_db.
 
 Section rel_semantics.
 
-  Variable (sym : Type) (sym_ar : sym -> nat) (X : Type)
-           (M : Type) (sem_sym : forall s, vec M (sym_ar s) -> M -> Prop).
+  Variable (Σ : fo_signature) (X : Type)
+           (sem_sym : forall s, vec X (ar_syms Σ s) -> X -> Prop).
 
-  Notation 𝕋 := (fo_term X sym_ar).
+  Notation 𝕋 := (fol_term Σ).
 
-  Implicit Type φ : X -> M -> Prop.
+  Implicit Type φ : nat -> X -> Prop.
 
-  Fixpoint fo_term_rsem φ (t : 𝕋) : M -> Prop :=
+  Fixpoint fo_term_rsem φ (t : 𝕋) : X -> Prop :=
     match t with
       | in_var x   => φ x
       | in_fot s v => fun m => exists w, @sem_sym s w m /\ forall p, fo_term_rsem φ (vec_pos v p) (vec_pos w p)
@@ -585,36 +350,6 @@ Section rel_semantics.
        <-> exists w, @sem_sym s w r 
                   /\ forall p, ⟦vec_pos v p⟧ φ (vec_pos w p).
   Proof. simpl; tauto. Qed.
-
-  (*
-
-  Definition fo_term_rsem φ : 𝕋 -> M -> Prop.
-  Proof.
-    induction 1 as [ x | s _ w ] using fo_term_recursion.
-    + exact (φ x).
-    + intros r.
-      exact (exists v, @sem_sym s v r /\ forall p, vec_pos w p (vec_pos v p)). 
-  Defined.
-
-  Notation "⟦ t ⟧" := (fun φ => @fo_term_rsem φ t).
-
-  Fact fo_term_rsem_fix_0 φ n : ⟦in_var n⟧ φ = φ n.
-  Proof. apply fo_term_recursion_fix_0. Qed.
-
-  Fact fo_term_rsem_fix_1 φ s v r : 
-           ⟦in_fot s v⟧ φ r 
-       <-> exists w, @sem_sym s w r 
-                  /\ forall p, ⟦vec_pos v p⟧ φ (vec_pos w p).
-  Proof.
-    unfold fo_term_rsem at 1; rewrite fo_term_recursion_fix_1.
-    apply exists_equiv; intros w.
-    apply fol_bin_sem_ext with (b := fol_conj); try tauto.
-    apply forall_equiv; intros p.
-    rewrite vec_pos_map.
-    apply fol_equiv_ext; auto.
-  Qed.
-
-  *)
 
   Opaque fo_term_rsem.
 
@@ -644,16 +379,16 @@ Hint Rewrite fo_term_rsem_fix_0 fo_term_rsem_fix_1 : fo_term_db.
 
 Section equiv.
 
-  Variable (sym : Type) (sym_ar : sym -> nat) (X : Type)
-           (M : Type) (sM : forall s, vec M (sym_ar s) -> M).
+  Variable (Σ : fo_signature) 
+           (X : Type) (M : fo_model Σ X).
 
-  Theorem fo_term_sem_rsem_equiv (t : fo_term X sym_ar) φ r : 
-           r = fo_term_sem sM φ t <-> fo_term_rsem (fun s v r => r = @sM s v) (fun n r => r = φ n) t r.
+  Theorem fo_term_sem_rsem_equiv (t : fol_term Σ) φ r : 
+           r = fo_term_sem M φ t <-> fo_term_rsem (fun s v r => r = fom_syms M s v) (fun n r => r = φ n) t r.
   Proof.
     revert φ r; induction t as [ n | s v IHv ]; intros phi r; rew fot; try tauto.
     split.
     + intros ->.
-      exists (vec_map (fo_term_sem sM phi) v); split; auto.
+      exists (vec_map (fo_term_sem M phi) v); split; auto.
       intros p; apply IHv; rew vec.
     + intros (w & -> & Hw); f_equal.
       apply vec_pos_ext; intros p; rew vec.
@@ -664,25 +399,26 @@ End equiv.
 
 Section rel_simulation.
 
-  Variable (sym : Type) (sym_ar : sym -> nat) (X : Type)
-           (M : Type) (sM : forall s, vec M (sym_ar s) -> M -> Prop)
-           (N : Type) (sN : forall s, vec N (sym_ar s) -> N -> Prop).
+  Variable (Σ : fo_signature)
+           (X : Type) (sX : forall s, vec X (ar_syms Σ s) -> X -> Prop)
+           (Y : Type) (sY : forall s, vec Y (ar_syms Σ s) -> Y -> Prop)
+           .
 
-  Notation 𝕋 := (fo_term X sym_ar).
+  Notation 𝕋 := (fol_term Σ).
 
-  Implicit Type (φ : X -> M -> Prop) (ψ : X -> N -> Prop).
+  Implicit Type (φ : nat -> X -> Prop) (ψ : nat -> Y -> Prop).
 
-  Variable (simul : M -> N -> Prop).
+  Variable (simul : X -> Y -> Prop).
 
   Infix "⋈" := simul (at level 70, no associativity).
   
-  Theorem fo_term_rsem_simul (t : fo_term X sym_ar) φ ψ :
+  Theorem fo_term_rsem_simul (t : fol_term  Σ) φ ψ :
              (forall n x y, In n (fo_term_vars t) -> x ⋈ y -> φ n x <-> ψ n y)
-          -> (forall s, In s (fo_term_syms t) -> forall x v y, x ⋈ y -> sM v x -> exists w, @sN s w y 
+          -> (forall s, In s (fo_term_syms t) -> forall x v y, x ⋈ y -> sX _ v x -> exists w, @sY s w y 
                                                                                          /\ forall p, vec_pos v p ⋈ vec_pos w p) 
-          -> (forall s, In s (fo_term_syms t) -> forall x w y, x ⋈ y -> sN w y -> exists v, @sM s v x 
+          -> (forall s, In s (fo_term_syms t) -> forall x w y, x ⋈ y -> sY _ w y -> exists v, @sX s v x 
                                                                                          /\ forall p, vec_pos v p ⋈ vec_pos w p)   
-          -> forall x y, x ⋈ y -> fo_term_rsem sM φ t x <-> fo_term_rsem sN ψ t y.
+          -> forall x y, x ⋈ y -> fo_term_rsem sX φ t x <-> fo_term_rsem sY ψ t y.
   Proof.
     induction t as [ n | s v IHv ]; intros H1 H2 H2' x y Hxy; rew fot; try tauto.
     + apply H1; simpl; auto.
